Veir/Passes/Matching/Builtin/Basic.lean
@@ -1,0 +1,13 @@
+module
+
+public import Veir.Passes.Matching.Basic
+
+public section
+
+/-! This file contains helper functions to match Builtin operations when defining a rewrite. -/
+
+namespace Veir
+
+def matchCastOp (op : OperationPtr) (ctx : IRContext OpCode) : Option ValuePtr := do
+  let (op, _) ← matchOp op ctx (.builtin .unrealized_conversion_cast) 1
+  return op[0]!
