Veir/Passes/Matching/Builtin/Lemmas.lean
@@ -1,0 +1,21 @@
+module
+
+public import Veir.Passes.Matching.Builtin.Basic
+
+import all Veir.Passes.Matching.Builtin.Basic
+
+public section
+
+/-! This file contains lemmas that characterize the behavior of the Builtin matching functions. -/
+
+namespace Veir
+
+/-- What matching `builtin.unrealized_conversion_cast` (via `matchCastOp`) syntactically guarantees. -/
+theorem matchCastOp_implies {op : OperationPtr} {ctx : IRContext OpCode} {operand} :
+    matchCastOp op ctx = some operand →
+    op.getOpType! ctx = .builtin .unrealized_conversion_cast ∧
+    op.getNumResults! ctx = 1 ∧
+    op.getOperands! ctx = #[operand] := by
+  intro hmatch
+  simp only [matchCastOp, bind, Option.bind, pure] at hmatch
+  grind
